\documentclass{article}
\usepackage[fleqn]{amsmath}
\begin{document}
\centerline{\sc \large \underline{Uncertainty Assignement - SPH 3U3}}
\centerline{\sc Andrey Khesin and Noah Cassidy}
\centerline{}

\begin{enumerate}
\item 
\item
\begin{enumerate}
\item
\begin{align*}
f &= x_1 + x_2\\
&= (10.005 \pm .003)\text{ cm} + (20.06 \pm .03)\text{ cm}\\
\sigma_{f} &= \sqrt{(\frac{\partial f}{\partial x_1})^2\sigma_{x_1}^2 + (\frac{\partial f}{\partial x_2})^2\sigma_{x_2}^2}\\
&= \sqrt{(1)^2(.003)^2 + (1)^2(.03)^2}\\
&= \sqrt{1(.000009) + 1(.0009)}\\
&= \sqrt{.000009 + .0009}\\
&= \sqrt{.0009}\\
&= .03\\
f &= (10.005 \pm .003)\text{ cm} + (20.06 \pm .03)\text{ cm}\\
&= (10.005 + 20.06 \pm \sigma_{f})\text{ cm}\\
&= (30.07 \pm .03)\text{ cm}
\end{align*}
\item
\begin{align*}
f &= x_1 - x_2\\
&= (352.1 \pm .9)\text{ m} - (162.36 \pm .05)\text{ m}\\
\sigma_{f} &= \sqrt{(\frac{\partial f}{\partial x_1})^2\sigma_{x_1}^2 + (\frac{\partial f}{\partial x_2})^2\sigma_{x_2}^2}\\
&= \sqrt{(1)^2(.9)^2 + (-1)^2(.05)^2}\\
&= \sqrt{1(.8) + 1(.003)}\\
&= \sqrt{.8 + .003}\\
&= \sqrt{.8}\\
&= .9\\
f &= (352.1 \pm .9)\text{ m} - (162.36 \pm .05)\text{ m}\\
&= (352.1 - 162.36 \pm \sigma_{f})\text{ m}\\
&= (189.7 \pm .9)\text{ m}
\end{align*}
\item
\begin{align*}
f &= x_1 + x_2\\
&= (56.7 \pm .2)\text{ cm} + (93.48 \pm .01)\text{ m}\\
\sigma_{f} &= \sqrt{(\frac{\partial f}{\partial x_1})^2\sigma_{x_1}^2 + (\frac{\partial f}{\partial x_2})^2\sigma_{x_2}^2}\\
&= \sqrt{(1)^2(.2)^2 + (1)^2(1)^2}\\
&= \sqrt{1(.04) + 1(1)}\\
&= \sqrt{.04 + 1}\\
&= \sqrt1\\
&= 1\\
f &= (56.7 \pm .2)\text{ cm} + (93.48 \pm .01)\text{ m}\\
&= (56.7 \pm .2)\text{ cm} + (9348 \pm 1)\text{ cm}\\
&= (56.7 + 9348 \pm \sigma_{f})\text{ cm}\\
&= (9410 \pm 1)\text{ cm}
\end{align*}
\item
\begin{align*}
f &= x_1 + x_2 - x_3\\
&= (14.5 \pm .2)\text{ mm} \pm (14.5 + .2)\text{ mm } - (23.1 \pm .1)\text{ mm}\\
\sigma_{f} &= \sqrt{(\frac{\partial f}{\partial x_1})^2\sigma_{x_1}^2 + (\frac{\partial f}{\partial x_2})^2\sigma_{x_2}^2 + (\frac{\partial f}{\partial x_3})^2\sigma_{x_3}^2}\\
&= \sqrt{(1)^2(.2)^2 + (1)^2(.2)^2 + (-1)^2(.1)^2}\\
&= \sqrt{1(.04) + 1(.04) + 1(.01)}\\
&= \sqrt{.04 + .04 + .01}\\
&= \sqrt{.09}\\
&= .3\\
f &= (14.5 \pm .2)\text{ mm} \pm (14.5 + .2)\text{ mm } - (23.1 \pm .1)\text{ mm}\\
&= (14.5 + 14.5 - 23.1 \pm \sigma_{f})\text{ mm}\\
&= (5.9 \pm .3)\text{ mm}
\end{align*}
\end{enumerate}
\item
\begin{enumerate}
\item
\begin{align*}
f &= x_1 * x_2\\
&= (23.56 \pm .05)\text{ kmh}^{-1} * (56.3 \pm .4)\text{ h}\\
\sigma_{f} &= \sqrt{(\frac{\partial f}{\partial x_1})^2\sigma_{x_1}^2 + (\frac{\partial f}{\partial x_2})^2\sigma_{x_2}^2}\\
&= \sqrt{(x_2)^2(.05)^2 + (x_1)^2(.4)^2}\\
&= \sqrt{(56.3)^2(.003) + (23.56)^2(.2)}\\
&= \sqrt{3170(.003) + 555.1(.2)}\\
&= \sqrt{10 + 100}\\
&= \sqrt{100}\\
&= 10\\
f &= (23.56 \pm .05)\text{ kmh}^{-1} * (56.3 \pm .4)\text{ h}\\
&= (23.56 * 56.3 \pm \sigma_{f})\text{ km}\\
&= (1330 \pm 9)\text{ km}\\
\end{align*}
\item
\begin{align*}
f &= \frac{x_1}{x_2}\\
&= \frac{(15.745 \pm .006)\text{ m}}{(0.36 \pm .05)\text{ m}}\\
\sigma_{f} &= \sqrt{(\frac{\partial f}{\partial x_1})^2\sigma_{x_1}^2 + (\frac{\partial f}{\partial x_2})^2\sigma_{x_2}^2}\\
&= \sqrt{(\frac1{x_2})^2(.006)^2 + (\frac{-x_1}{x_2^2})^2(.05)^2}\\
&= \sqrt{(\frac1{0.36})^2(.00004) + (\frac{-15.745}{0.36^2})^2(.003)}\\
&= \sqrt{(2.8)^2(.00004) + (\frac{-15.745}{0.13})^2(.003)}\\
&= \sqrt{7.8(.00004) + (-120)^2(.003)}\\
&= \sqrt{0.0003 + 14000(.003)}\\
&= \sqrt{0.0003 + 40}\\
&= \sqrt{40}\\
&= 6\\
f &= \frac{(15.745 \pm .006)\text{ m}}{(0.36 \pm .05)\text{ m}}\\
&= \frac{15.745}{0.36} \pm \sigma_{f}\\
&= 44 \pm 6
\end{align*}
\item
\begin{align*}
f &= 2x_1\\
&= 2(1.63 \pm .03)\text{ mm}\\
\sigma_{f} &= \sqrt{(\frac{\partial f}{\partial x_1})^2\sigma_{x_1}^2}\\
&= 2(.03)\\
&= .06\\
f &= 2(1.63 \pm .03)\text{ mm}\\
&= 2(1.63) \pm \sigma_{f}\text{ mm}\\
&= 3.26 \pm .06\text{ mm}\\
\end{align*}
\item
\begin{align*}
f &= \frac{x_1x_2}{x_3}\\
&= \frac{(1.23 \pm .02)\text{ ms}^{-1} * (2.637 \pm .003)\text{ ms}^{-1}}{(5.6 \pm .1)\text{ ms}^{-1}}\\
\sigma_{f} &= \sqrt{(\frac{\partial f}{\partial x_1})^2\sigma_{x_1}^2 + (\frac{\partial f}{\partial x_2})^2\sigma_{x_2}^2 + (\frac{\partial f}{\partial x_3})^2\sigma_{x_3}^2}\\
&= \sqrt{(\frac{x_2}{x_3})^2(.02)^2 + (\frac{x_1}{x_3})^2(.003)^2 + (\frac{-x_1x_2}{x_3^2})^2(.1)^2}\\
&= \sqrt{(\frac{2.637}{5.6})^2(.0004) + (\frac{1.23}{5.6})^2(.000009) + (\frac{-1.23(2.637)}{5.6^2})^2(.01)}\\
&= \sqrt{(.47)^2(.0004) + (.22)^2(.000009) + (\frac{-3.24}{31.36})^2(.01)}\\
&= \sqrt{.22(.0004) + .048(.000009) + (-.103)^2(.01)}\\
&= \sqrt{.00009 + .0000004 + .0107)(.01)}\\
&= \sqrt{.00009 + .0001}\\
&= \sqrt{.0002}\\
&= .01\\
f &= \frac{(1.23 \pm .02)\text{ ms}^{-1} * (2.637 \pm .003)\text{ ms}^{-1}}{(5.6 \pm .1)\text{ ms}^{-1}}\\
&= (\frac{1.23 * 2.637}{5.6} \pm \sigma_{f})\text{ ms}^{-1}\\
&= (.58 \pm .01)\text{ ms}^{-1}
\end{align*}
\end{enumerate}
\item
\begin{enumerate}
\item
\begin{align*}
f &= x_1 + \frac{2x_2}{x_3}\\
&= (61.12 \pm .05)\text{ cm} + \frac{2(45.23 \pm .06)\text{ cm}^2}{(1.03 \pm .04)\text{ cm}}\\
\sigma_{f} &= \sqrt{(\frac{\partial f}{\partial x_1})^2\sigma_{x_1}^2 + (\frac{\partial f}{\partial x_2})^2\sigma_{x_2}^2 + (\frac{\partial f}{\partial x_3})^2\sigma_{x_3}^2}\\
&= \sqrt{(1)^2(.05)^2 + (\frac2{x_3})^2(.06)^2 + (\frac{-2x_2}{x_3^2})^2(.04)^2}\\
&= \sqrt{1(.003) + (\frac2{1.03})^2(.004) + (\frac{-2(45.23)}{1.03^2})^2(.002)}\\
&= \sqrt{.003 + (\frac2{1.03})^2(.004) + (\frac{-2(45.23)}{1.03^2})^2(.002)}\\
&= \sqrt{.003 + (2)^2(.004) + (\frac{-90.46}{1.06})^2(.002)}\\
&= \sqrt{.003 + 4(.004) + (-85.3)^2(.002)}\\
&= \sqrt{.003 + .02 + 7280(.002)}\\
&= \sqrt{.02 + 15}\\
&= \sqrt{15}\\
&= 4\\
f &= (61.12 \pm .05)\text{ cm} + \frac{2(45.23 \pm .06)\text{ cm}^2}{(1.03 \pm .04)\text{ cm}}\\
&= (61.12 + \frac{2(45.23)}{1.03} \pm \sigma_{f})\text{ cm}\\
&= (61.12 + \frac{90.46}{1.03} \pm 3)\text{ cm}\\
&= (61.21 + 87.8252 \pm 3)\text{ cm}\\
&= (148.9 \pm 3)\text{ cm}\\
&= (149 \pm 3)\text{ cm}
\end{align*}
\item
\begin{align*}
f &= x_1x_2 - x_3\\
&= (1005.1 \pm .2)\text{ kmh}^{-1} * (3.93 \pm .02)\text{ kmh}^{-1} - (583.68 \pm .06)\text{ km}^2\text{h}^{-2}\\
\sigma_{f} &= \sqrt{(\frac{\partial f}{\partial x_1})^2\sigma_{x_1}^2 + (\frac{\partial f}{\partial x_2})^2\sigma_{x_2}^2 + (\frac{\partial f}{\partial x_3})^2\sigma_{x_3}^2}\\
&= \sqrt{(x_2)^2(.2)^2 + (x_1)^2(.02)^2 + (-1)^2(.06)^2}\\
&= \sqrt{(3.93)^2(.2)^2 + (1005.1)^2(.02)^2 + 1(.0004)}\\
&= \sqrt{15.4(.04) + 1010200(.0004) + .0004}\\
&= \sqrt{.6 + 400 + .0004}\\
&= \sqrt{400}\\
&= 20\\
f &= (1005.1 \pm .2)\text{ kmh}^{-1} * (3.93 \pm .02)\text{ kmh}^{-1} - (583.68 \pm .06)\text{ km}^2\text{h}^{-2}\\
&= (1005.1 * 3.93 - 583.68 \pm \sigma_{f})\text{ km}^2\text{h}^{-2}\\
&= (3370 \pm 20)\text{ km}^2\text{h}^{-2}\\
\end{align*}
\end{enumerate}
\item
\begin{enumerate}
\item
\begin{align*}
y &= x_1^2\sin(x_1x_2)\\
&= (1.23 \pm .04)^2\sin((1.23 \pm .04) * (1.99 \pm .01))\\
\sigma_{y} &= \sqrt{(\frac{\partial y}{\partial x_1})^2\sigma_{x_1}^2 + (\frac{\partial y}{\partial x_2})^2\sigma_{x_2}^2}\\
&= \sqrt{(2x_1\sin(x_1x_2) + x_1^2x_2\cos(x_1x_2))^2(.04)^2 + (x_1^3\cos(x_1x_2))^2(.01)^2}\\
&= ((2(1.23)\sin(1.23(1.99)) + .002(1.23)^2(1.99)\cos(1.23(1.99)))^2 +\\
&+ .0001((1.23)^3\cos(1.23(1.99)))^2)^\frac12\\
&= \sqrt{(2.46\sin(2.45) + 1.51(.004)\cos(2.45))^2 + .0001(1.86\cos(2.45))^2}\\
&= \sqrt{(2.46(.638) + .006(-.770))^2 + .0001(1.86(-.770))^2}\\
&= \sqrt{(1.57 - .005)^2 + .0001(-1.43)^2}\\
&= \sqrt{(2)^2 + .0001(2.04)}\\
&= \sqrt{4 + .0002}\\
&= \sqrt{4}\\
&= 2\\
y &= (1.23 \pm .04)^2\sin((1.23 \pm .04) * (1.99 \pm .01))\\
&= (1.23)^2\sin(1.23(1.99)) \pm \sigma_{y}\\
&= 1.51\sin(2.45) \pm 2\\
&= 1.51(.638) \pm 2\\
&= 0.963 \pm 2\\
&= 1 \pm 2
\end{align*}
\item
\begin{align*}
y &= x_1^2x_2^3e^{x_1x_2} + x_1^2x_2\\
&= (1.23 \pm .04)^2 * (1.99 \pm .01)^3e^{(1.23 \pm .04) * (1.99 \pm .01)} + (1.23 \pm .04)^2 * (1.99 \pm .01)\\
\sigma_{y} &= \sqrt{(\frac{\partial y}{\partial x_1})^2\sigma_{x_1}^2 + (\frac{\partial y}{\partial x_2})^2\sigma_{x_2}^2}\\
&= \sqrt{(2x_1x_2^3e^{x_1x_2} + x_1^2x_2^4e^{x_1x_2} + 2x_1x_2)^2(.04)^2 + (3x_1^2x_2^2e^{x_1x_2} + x_1^3x_2^3e^{x_1x_2} + x_1^2)^2(.01)^2}\\
&= ((2(1.23)(1.99)^3e^{1.23(1.99)} + (1.23)^2(1.99)^4e^{1.23(1.99)} + 2(1.23)(1.99))^2(.002) +\\
&+ (3(1.23)^2(1.99)^2e^{1.23(1.99)} + (1.23)^3(1.99)^3e^{1.23(1.99)} + (1.23)^2)^2(.0001))^{\frac{1}{2}}\\
&= ((2.46(7.88)e^{2.45} + 1.51(15.7)e^{2.45} + 4.90)^2(.002) + (3(1.51)(3.96)e^{2.45} +\\
&+ 1.86(7.88)e^{2.45} + 1.51)^2(.0001))^{\frac{1}{2}}\\
&= \sqrt{(19.4(11.6) + 23.7(11.6) + 4.90)^2(.002) + (17.9(11.6) + 14.7(11.6) + 1.51)^2(.0001)}\\
&= \sqrt{(225 + 275 + 4.90)^2(.002) + (208 + 171 + 1.51)^2(.0001)}\\
&= \sqrt{(505)^2(.002) + (381)^2(.0001)}\\
&= \sqrt{255000(.002) + 145000(.0001)}\\
&= \sqrt{500 + 10}\\
&= \sqrt{500}\\
&= 20\\
y &= (1.23 \pm .04)^2 * (1.99 \pm .01)^3e^{(1.23 \pm .04) * (1.99 \pm .01)} + (1.23 \pm .04)^2 * (1.99 \pm .01)\\
&= (1.23)^2(1.99)^3e^{1.23(1.99)} + 1.99(1.23)^2 \pm \sigma_{y}\\
&= 1.51(7.88)e^{2.45} + 1.99(1.51) \pm 20\\
&= 138 + 3 \pm 20\\
&= 141 \pm 20\\
&= 140 \pm 20
\end{align*}
\end{enumerate}
\end{enumerate}
\end{document}
